LeanLgtm/Arrays.lean
@@ -1,0 +1,311 @@
+import LeanLgtm.XSimp
+import LeanLgtm.XChange
+import LeanLgtm.Util
+import LeanLgtm.SepLog
+
+
+/- ============== Definitions for Arrays ============== -/
+
+open val
+open trm
+
+def hheader (n : Int) (p : loc) : hprop :=
+  p ~~> (val_int n)
+
+lemma hheader_eq p n :
+  (hheader n p) = (p ~~> (val_int n)) := by
+  sdone
+
+def hcell (v : val) (p : loc) (i : Int) : hprop :=
+  ((p + 1 + (Int.natAbs i)) ~~> v) ∗ ⌜i >= 0⌝
+
+lemma hcell_eq v p i :
+  (hcell v p i) = ((p + 1 + (Int.natAbs i)) ~~> v) ∗ ⌜i >= 0⌝ := by
+  sdone
+
+lemma hcell_nonneg v p i :
+  hcell v p i ==> hcell v p i ∗ ⌜i >= 0⌝ := by
+  sby srw hcell_eq ; xsimp
+
+def hseg (L : List val) (p : loc) (j : Int) : hprop :=
+  match L with
+  | []      => emp
+  | x :: L' => (hcell x p j) ∗ (hseg L' p (j + 1))
+
+def harray (L : List val) (p : loc) : hprop :=
+  hheader (L.length) p ∗ hseg L p 0
+
+lemma harray_eq p L :
+  harray L p = h∃ n, ⌜n = L.length⌝ ∗ hheader n p ∗ hseg L p 0 := by
+  sby srw harray ; xsimp ; xsimp
+
+/- inversion lemma for hseg -/
+
+lemma hseg_start_eq L p j1 j2 :
+  j1 = j2 →
+  hseg L p j1 ==> hseg L p j2 := by
+  sdone
+
+
+/- ================== Implementation of Arrays ================= -/
+
+/- A simplified specification for non-negative pointer addition -/
+
+lemma natabs_nonneg (p : Nat) (n : Int) :
+  n ≥ 0 → (p + n).natAbs = p + n.natAbs := by
+  omega
+
+lemma triple_ptr_add_nonneg (p : loc) (n : Int) :
+  n >= 0 →
+  triple (trm_app prim.val_ptr_add p n)
+    emp
+    (fun r ↦ ⌜r = val_loc (p + Int.natAbs n)⌝) := by
+  move=> ?
+  apply (triple_conseq _ emp
+    (fun r ↦ ⌜r = val_loc (Int.toNat (Int.natAbs (p + n)))⌝))
+  apply triple_ptr_add
+  { omega }
+  { xsimp }
+  xsimp ; xsimp ; subst r=> /==
+  sby apply natabs_nonneg
+
+
+/- Semantics of Low-Level Block Allocation -/
+
+#check val_alloc
+
+#check eval.eval_alloc
+/- eval.eval_alloc (n : ℤ) (sa : state) (Q : val → state → Prop) :
+  n ≥ 0 →
+  (∀ (p : loc) (sb : state),
+      sb = conseq val (make_list n.natAbs val_uninit) p →
+      p ≠ null →
+      Finmap.Disjoint sa sb →
+      Q p (sb ∪ sa)) →
+      eval sa (trm_app val_aloc n) Q
+ -/
+
+/- Heap predicate for describing a range of cells -/
+
+def hrange (L : List val) (p : loc) : hprop :=
+  match L with
+  | []      => emp
+  | x :: L' => (p ~~> x) ∗ (hrange L' (p + 1))
+
+lemma hrange_intro L p :
+  (hrange L p) (conseq L p) := by
+  induction L generalizing p ; srw conseq hrange=> //
+  apply hstar_intro=>//
+  sby apply disjoint_single_conseq
+
+lemma triple_alloc (n : Int) :
+  n ≥ 0 →
+  triple (trm_app val_alloc n)
+    emp
+    (funloc p ↦ hrange (make_list n.natAbs val_uninit) p ∗ ⌜p ≠ null⌝ ) := by
+  move=> ?? [] ; apply eval.eval_alloc=>// > *
+  apply (hexists_intro _ p)
+  srw hstar_hpure_l Finmap.union_empty hstar_hpure_r => ⟨|⟨|⟩⟩ //
+  subst sb ; apply hrange_intro
+
+
+/- Low-level Implementation of arrays -/
+
+def val_array_length : val := [lang|
+  fun p => !p ]
+
+def val_array_get : val := [lang|
+  fun p i =>
+    let p1 := val_ptr_add p 1 in
+    let q := val_ptr_add p1 i in
+    !q ]
+
+def val_array_set : val := [lang|
+  fun p i v =>
+    let p1 := val_ptr_add p 1 in
+    let q := val_ptr_add p1 i in
+    q := v ]
+
+def val_array_fill : val := [lang|
+  fix f p i n v =>
+    let b := n > 0 in
+    if b then
+      val_array_set p i v ;
+      let m := n - 1 in
+      let j := i + 1 in
+      f p j m v
+    end ]
+
+def val_array_make : val := [lang|
+  fun n v =>
+    let m := n + 1 in
+    let p := val_alloc m in
+    val_set p n ;
+    val_array_fill p 0 n v ;
+    p ]
+
+/- ==================== Properties of Arrays ==================== -/
+
+/- properties of [hseg] -/
+
+lemma hseg_nil p j :
+  hseg [] p j = emp := by
+  sdone
+
+lemma hseg_one v p j :
+  hseg (v :: []) p j = hcell v p j := by
+  sby srw hseg hseg ; xsimp
+
+lemma hseg_cons v p j L :
+  hseg (v :: L) p j = hcell v p j ∗ hseg L p (j + 1) := by
+  sby srw hseg
+
+lemma hseg_app L1 L2 p j :
+  hseg (L1 ++ L2) p j =
+  hseg L1 p j ∗ hseg L2 p (j + L1.length) := by
+  induction L1 generalizing j with
+  | nil         => srw hseg /== ; hsimp
+  | cons _ _ ih =>
+      sby dsimp ; srw ?hseg_cons ih -[4](add_comm 1) add_assoc ; hsimp
+
+
+/- ------------------- Focus lemmas for [hseg] ------------------- -/
+
+lemma list_cons_length (A : Type) (x : A) (L : List A) :
+  (x :: L).length = 1 + L.length := by
+  simp
+  omega
+
+#check List.append_of_mem
+lemma list_middle_inv (A : Type) (n : Nat) (l : List A) :
+  n < l.length →
+  exists (x : A) (l1 l2 : List A),
+    l = l1 ++ x :: l2 ∧ l1.length = n := by
+  induction n generalizing l with
+  | zero       => move=> ? ; cases l => //
+  | succ n' ih =>
+      move=> hlen ; cases l with
+      | nil => sdone
+      | cons x l' =>
+          have h : (n' < l'.length) := by srw list_cons_length at hlen ; omega
+          apply ih in h=> [x' [l1 [l2]]] ?
+          exists x', (x :: l1), l2 ; sdone
+
+#check List.getElem_of_append
+lemma nth_middle (A : Type) (IA : Inhabited A) (n : Nat)
+  (l1 l2 : List A) (x : A) :
+  n = l1.length → (l1 ++ x :: l2)[n]! = x := by sorry
+
+#check List.concat_eq_append
+lemma update_middle (A : Type) (IA : Inhabited A) (n : Nat)
+  (l1 l2 : List A) (x v : A) :
+  n = l1.length → (l1 ++ x :: l2).set n v = (l1.concat v) ++ l2 := by sorry
+
+lemma hseg_focus_relative (k : Nat) L p j :
+  0 <= k ∧ k < L.length →
+  hseg L p j ==>
+  hcell L[k]! p (j + k)
+    ∗ (h∀ w, hcell w p (j + k) -∗ hseg (L.set k w) p j) := by
+  move=> [] ? /list_middle_inv ![> ?] hlen
+  move: (Eq.symm hlen) => /nth_middle hmid
+  subst L ; srw (hmid _ w_2 w) hseg_app hseg_cons hlen -hstar_comm_assoc
+  apply himpl_frame_r
+  apply himpl_hforall_r => ?
+  move: (Eq.symm hlen) => /(update_middle val _ k w_1 w_2 w) hset
+  srw (hset _) ?List.concat_append ?hseg_app ?hseg_cons ?hlen
+  sby xsimp
+
+lemma add_Int.natAbs i j :
+  0 <= i - j → j + Int.natAbs (i - j) = i := by omega
+
+lemma hseg_focus (i j : Int) L p :
+  0 <= i - j ∧ i - j < L.length →
+  hseg L p j ==>
+  hcell L[Int.natAbs (i - j)]! p i
+    ∗ (h∀ w, hcell w p i -∗ hseg (L.set (Int.natAbs (i - j)) w) p j) := by
+  move=> [] * ; xchange (hseg_focus_relative (Int.natAbs (i - j))) ; omega
+  sby srw add_Int.natAbs ; xsimp
+
+lemma harray_focus i L p :
+  0 <= i ∧ i < L.length →
+  harray L p ==>
+  hcell L[Int.natAbs i]! p i
+    ∗ (h∀ w, hcell w p i -∗ harray (L.set (Int.natAbs i) w) p) := by
+  move=> [] *
+  srw ?harray ; xchange (hseg_focus i) ; omega ; simp
+  apply himpl_frame_r ; apply himpl_hforall_r => x
+  xchange (hforall_specialize _ x)
+  xsimp
+
+lemma set_nth_same (A : Type) (IA : Inhabited A) (n : Nat) (l : List A) :
+  n < l.length → l.set n l[n]! = l := by sorry
+
+lemma harray_focus_read i L p :
+  0 <= i ∧ i < L.length →
+  harray L p ==>
+  hcell L[Int.natAbs i]! p i ∗ (hcell L[Int.natAbs i]! p i -∗ harray L p) := by
+  move=> [] *
+  xchange (harray_focus i L p) => // ; xsimp
+  xchange (hforall_specialize _ L[Int.natAbs i]!)
+  srw set_nth_same
+  xsimp
+  omega
+
+
+/- ========================= Triple rules for Arrays ========================= -/
+
+lemma triple_array_make n (v : val) :
+  n >= 0 →
+  triple (trm_app val_array_make (val_int n) v)
+    emp
+    (funloc p ↦ harray (make_list (Int.natAbs n) v) p) := by sorry
+
+lemma triple_array_length L (p : loc) :
+  triple (trm_app val_array_length p)
+    (harray L p)
+    (fun r ↦ ⌜r = L.length⌝ ∗ harray L p) := by sorry
+
+lemma triple_array_get L (p : loc) (i : Int) :
+   0 <= i ∧ i < L.length →
+   triple (trm_app val_array_get p i)
+    (harray L p)
+    (fun r ↦ ⌜r = L[Int.natAbs i]!⌝ ∗ harray L p) := by sorry
+
+lemma triple_array_set L (p : loc) (i : Int) (v : val) :
+  0 <= i ∧ i < L.length →
+  triple (trm_app val_array_set p i v)
+    (harray L p)
+    (fun _ ↦ harray (L.set (Int.natAbs i) v) p) := by sorry
+
+lemma triple_array_length_hheader (n : Int) (p : loc) :
+  triple (trm_app val_array_length p)
+    (hheader n p)
+    (fun r ↦ ⌜r = n⌝ ∗ hheader n p) := by sorry
+
+lemma triple_array_get_hcell (p : loc) (i : Int) (v : val) :
+  triple (trm_app val_array_get p i)
+    (hcell v p i)
+    (fun r ↦ ⌜r = v⌝ ∗ hcell v p i) := by sorry
+
+lemma triple_array_set_hcell (p : loc) (i : Int) (v w : val) :
+  triple (trm_app val_array_set p i v)
+    (hcell w p i)
+    (fun _ ↦ hcell v p i) := by sorry
+
+lemma triple_array_make_hseg (n : Int) (v : val) :
+  n >= 0 →
+  triple (trm_app val_array_make n v)
+    emp
+    (funloc p ↦ hheader (Int.natAbs n) p ∗ hseg (make_list (Int.natAbs n) v) p 0) := by sorry
+
+lemma triple_array_get_hseg L (p : loc) (i j : Int) :
+  0 <= i - j ∧ i - j < L.length →
+  triple (trm_app val_array_get p i)
+    (hseg L p j)
+    (fun r ↦ ⌜r = L[Int.natAbs (i - j)]!⌝ ∗ hseg L p j) := by sorry
+
+lemma triple_array_set_hseg L (p : loc) (i j : Int) (v : val) :
+  0 <= i - j ∧ i - j < L.length →
+  triple (trm_app val_array_set p i v)
+    (hseg L p j)
+    (fun _ ↦ hseg (L.set (Int.natAbs (i - j)) v) p j) := by sorry
